@prefix : <https://w3id.org/miao#> .
@prefix owl: <http://www.w3.org/2002/07/owl#> .
@prefix rdf: <http://www.w3.org/1999/02/22-rdf-syntax-ns#> .
@prefix xml: <http://www.w3.org/XML/1998/namespace> .
@prefix xsd: <http://www.w3.org/2001/XMLSchema#> .
@prefix rdfs: <http://www.w3.org/2000/01/rdf-schema#> .
@base <https://w3id.org/miao#> .

<https://w3id.org/miao#> rdf:type owl:Ontology ;
                          owl:imports <http://www.w3.org/2016/03/mls#> ;
                          <http://purl.org/dc/terms/created> "2025-10-27"^^xsd:date ;
                          <http://purl.org/dc/terms/creator> "Carlos Á. Iglesias" ,
                                                             "Gianluca Apriceno" ,
                                                             "Mauro Dragoni" ,
                                                             "Sergio Muñoz López" ,
                                                             "Tania Bailoni" ;
                          <http://purl.org/dc/terms/license> "https://creativecommons.org/licenses/by-nc-sa/4.0/" ;
                          <http://purl.org/dc/terms/modified> "2025-10-27"^^xsd:date ;
                          <http://purl.org/dc/terms/publisher> "Intelligent Digital Agents Research Group <https://ida.fbk.eu> @digital health and wellbeing center, fondazione bruno kessler <https://digitalhealthcenter-en.fbk.eu/home>  and gsi - universidad politécnica de madrid <https://www.gsi.upm.es/es/>" ;
                          <http://purl.org/dc/terms/rights> "CreativeCommons 4.0 NonCommercial-ShareAlike <https://creativecommons.org/licenses/by-nc-sa/4.0/>" ;
                          <http://purl.org/dc/terms/title> "MIAO: A Mental Illness Analysis Ontology for Detecting Mental Health Conditions"@en ;
                          <http://purl.org/vocab/vann/preferredNamespacePrefix> "miao" ;
                          <http://purl.org/vocab/vann/preferredNamespaceUri> "https://w3id.org/miao#" ;
                          owl:versionInfo 1.00 .

#################################################################
#    Annotation properties
#################################################################

###  http://purl.org/dc/terms/created
<http://purl.org/dc/terms/created> rdf:type owl:AnnotationProperty .


###  http://purl.org/dc/terms/creator
<http://purl.org/dc/terms/creator> rdf:type owl:AnnotationProperty .


###  http://purl.org/dc/terms/license
<http://purl.org/dc/terms/license> rdf:type owl:AnnotationProperty .


###  http://purl.org/dc/terms/modified
<http://purl.org/dc/terms/modified> rdf:type owl:AnnotationProperty .


###  http://purl.org/dc/terms/publisher
<http://purl.org/dc/terms/publisher> rdf:type owl:AnnotationProperty .


###  http://purl.org/dc/terms/rights
<http://purl.org/dc/terms/rights> rdf:type owl:AnnotationProperty .


###  http://purl.org/dc/terms/title
<http://purl.org/dc/terms/title> rdf:type owl:AnnotationProperty .


###  http://purl.org/vocab/vann/preferredNamespacePrefix
<http://purl.org/vocab/vann/preferredNamespacePrefix> rdf:type owl:AnnotationProperty .


###  http://purl.org/vocab/vann/preferredNamespaceUri
<http://purl.org/vocab/vann/preferredNamespaceUri> rdf:type owl:AnnotationProperty .


#################################################################
#    Datatypes
#################################################################

###  http://purl.org/dc/terms/URI
<http://purl.org/dc/terms/URI> rdf:type rdfs:Datatype .


###  http://www.w3.org/2001/XMLSchema#date
xsd:date rdf:type rdfs:Datatype .


#################################################################
#    Object Properties
#################################################################

###  http://www.w3.org/ns/prov#generated
<http://www.w3.org/ns/prov#generated> rdf:type owl:ObjectProperty ;
                                      owl:inverseOf <http://www.w3.org/ns/prov#wasGeneratedBy> ;
                                      rdf:type owl:FunctionalProperty ;
                                      rdfs:domain :MentalIllnessesDetection ;
                                      rdfs:range :MentalIlnessesSet ;
                                      rdfs:comment "Relation taken from the Prov ontology that is used to represent the relation between a MentalIlnessesDetection and the generated set of MentalIllnessesSet." .


###  http://www.w3.org/ns/prov#wasGeneratedBy
<http://www.w3.org/ns/prov#wasGeneratedBy> rdf:type owl:ObjectProperty ,
                                                    owl:InverseFunctionalProperty ;
                                           rdfs:domain :MentalIlnessesSet ;
                                           rdfs:range :MentalIllnessesDetection ;
                                           rdfs:comment "Ref: https://www.w3.org/TR/prov-o/#wasGeneratedBy" .


###  https://w3id.org/miao#belongsToMentalIllnessesSet
:belongsToMentalIllnessesSet rdf:type owl:ObjectProperty ;
                             owl:inverseOf :hasMentalIllness ;
                             rdfs:domain :MentalIlness ;
                             rdfs:range :MentalIlnessesSet ;
                             rdfs:comment "Inverse relation of hasMentalIlness. This relation connect a MentalIllness with its corresponding MentalIlnessSet." .


###  https://w3id.org/miao#hasInputData
:hasInputData rdf:type owl:ObjectProperty ;
              owl:inverseOf :isInputOfMentalIlnessesDetection ;
              rdfs:domain :MentalIllnessesDetection ;
              rdfs:range <http://www.w3.org/ns/mls#Data> ;
              rdfs:comment "A relation between a MentalIllnessesDetection and data that is taken as input to the MentalIllnessesDetection." .


###  https://w3id.org/miao#hasMentalIllness
:hasMentalIllness rdf:type owl:ObjectProperty ;
                  rdfs:domain :MentalIlnessesSet ;
                  rdfs:range :MentalIlness ;
                  rdfs:comment "Relation connecting a MentalIllnessesSet with its corresponding MentalIlnesses." .


###  https://w3id.org/miao#hasMentalIlnessCategory
:hasMentalIlnessCategory rdf:type owl:ObjectProperty ;
                         owl:inverseOf :isMentalIlnessCategoryOf ;
                         rdfs:domain :MentalIlnessesSchema ;
                         rdfs:range :MentalIlnessCategory ;
                         rdfs:comment "A relation between a MentalIllnessesModel and its Mental Illness categories." .


###  https://w3id.org/miao#isInputOfMentalIlnessesDetection
:isInputOfMentalIlnessesDetection rdf:type owl:ObjectProperty ;
                                  rdfs:domain <http://www.w3.org/ns/mls#Data> ;
                                  rdfs:range :MentalIllnessesDetection .


###  https://w3id.org/miao#isMentalIlnessCategoryOf
:isMentalIlnessCategoryOf rdf:type owl:ObjectProperty ;
                          rdfs:domain :MentalIlnessCategory ;
                          rdfs:range :MentalIlnessesSchema ;
                          rdfs:comment "Inverse relation of hasMentalIllnessCategory object propery that represents the relation between a MentalIllnessCategory and its corresponding MentalIllnessesModel." .


###  https://w3id.org/miao#referredToMentalIllness
:referredToMentalIllness rdf:type owl:ObjectProperty ;
                         owl:inverseOf :referredToMentalIllnessCategory ;
                         rdf:type owl:InverseFunctionalProperty ;
                         rdfs:domain :MentalIlnessCategory ;
                         rdfs:range :MentalIlness ;
                         rdfs:comment "Inverse relation of referredToMentalIllnessCategory used to represent to which MentalIlness (predicted) a MentalIlnessCategoy (from the literature) corresponds to." .


###  https://w3id.org/miao#referredToMentalIllnessCategory
:referredToMentalIllnessCategory rdf:type owl:ObjectProperty ,
                                          owl:FunctionalProperty ;
                                 rdfs:domain :MentalIlness ;
                                 rdfs:range :MentalIlnessCategory ;
                                 rdfs:comment "Relation used to represent to which MentalIlnessCategoy (from the literature) a MentalIlness (predicted) corresponds to." .


###  https://w3id.org/miao#usedInMentalIllnessesDetection
:usedInMentalIllnessesDetection rdf:type owl:ObjectProperty ;
                                owl:inverseOf :usedMentalIllnessesSchema ;
                                rdfs:domain :MentalIlnessesSchema ;
                                rdfs:range :MentalIllnessesDetection ;
                                rdfs:comment "Inverse relation of usedMentalIlnessesSchema used to indicate which MentalIllnessesDetection a specific MentalIllnessesSchema (from the literature) refers to." .


###  https://w3id.org/miao#usedMentalIllnessesSchema
:usedMentalIllnessesSchema rdf:type owl:ObjectProperty ,
                                    owl:FunctionalProperty ;
                           rdfs:domain :MentalIllnessesDetection ;
                           rdfs:range :MentalIlnessesSchema ;
                           rdfs:comment "Relations used to indicate to which MentalIllnessesSchema (from the literature) a MentalIllnessesDetection is based on." .


#################################################################
#    Data properties
#################################################################

###  https://w3id.org/miao#hasMentalIllnessDetectionConfidence
:hasMentalIllnessDetectionConfidence rdf:type owl:DatatypeProperty ;
                                     rdfs:domain :MentalIlness ;
                                     rdfs:range xsd:decimal ;
                                     rdfs:comment "Data Property used to represent the confidence of both an human expert or a machine/deep learning model about the presence of a mental illness." .


###  https://w3id.org/miao#hasMentalIllnessLevel
:hasMentalIllnessLevel rdf:type owl:DatatypeProperty ;
                       rdfs:domain :MentalIlness ;
                       rdfs:range xsd:string ;
                       rdfs:comment "Represents the intensity of the mental illness as a categorical value, e.g., Low, Medium, or High." .


###  https://w3id.org/miao#hasMentalIllnessScore
:hasMentalIllnessScore rdf:type owl:DatatypeProperty ;
                       rdfs:domain :MentalIlness ;
                       rdfs:range xsd:decimal ;
                       rdfs:comment "Represents the intensity of the mental illness as a numeric score between 0 and 1." .


###  https://w3id.org/miao#refersToSample
:refersToSample rdf:type owl:DatatypeProperty ;
                rdfs:domain :MentalIlness ;
                rdfs:range xsd:string ;
                rdfs:comment "This data property represents the unique identifier of the specific data sample on which one or more mental illnesses have been detected. It is used to link a mental illness detection result to the original collected data instance." .


#################################################################
#    Classes
#################################################################

###  http://www.w3.org/ns/mls#Data
<http://www.w3.org/ns/mls#Data> rdf:type owl:Class .


###  http://www.w3.org/ns/mls#Run
<http://www.w3.org/ns/mls#Run> rdf:type owl:Class .


###  http://www.w3.org/ns/prov#Activity
<http://www.w3.org/ns/prov#Activity> rdf:type owl:Class ;
                                     rdfs:comment "Ref: https://www.w3.org/TR/prov-o/#Activity" .


###  http://www.w3.org/ns/prov#Entity
<http://www.w3.org/ns/prov#Entity> rdf:type owl:Class ;
                                   rdfs:comment "Ref: https://www.w3.org/TR/prov-o/#Entity" .


###  https://w3id.org/miao#AutomaticMentalIlnessesDetection
:AutomaticMentalIlnessesDetection rdf:type owl:Class ;
                                  rdfs:subClassOf <http://www.w3.org/ns/mls#Run> ,
                                                  :MentalIllnessesDetection ;
                                  owl:disjointWith :ManualMentalIllnessesDetection ;
                                  rdfs:comment "An AutomaticMentalIllnessesDetection represents an analysis (i.e., a run) performed by a machine/deep learning model to detect mental illnesses from a given source." ;
                                  rdfs:label "Automatic Mental Illnesses Detection"@en ,
                                             "Rilevamento Automatico Malattie Mentali"@it .


###  https://w3id.org/miao#ManualMentalIllnessesDetection
:ManualMentalIllnessesDetection rdf:type owl:Class ;
                                rdfs:subClassOf :MentalIllnessesDetection ;
                                rdfs:comment "A ManualMentalIllnessesDetection represents an analysis performed by a human expert to detect mental illnesses from a given source." ;
                                rdfs:label "Manual Detection Mental Illnesses"@en ,
                                           "Rilevamento Manuale Malattie Mentali"@it .


###  https://w3id.org/miao#MentalIllnessesDetection
:MentalIllnessesDetection rdf:type owl:Class ;
                          rdfs:subClassOf <http://www.w3.org/ns/prov#Activity> ,
                                          [ rdf:type owl:Restriction ;
                                            owl:onProperty :hasInputData ;
                                            owl:someValuesFrom <http://www.w3.org/ns/mls#Data>
                                          ] ,
                                          [ rdf:type owl:Restriction ;
                                            owl:onProperty <http://www.w3.org/ns/prov#generated> ;
                                            owl:qualifiedCardinality "1"^^xsd:nonNegativeInteger ;
                                            owl:onClass :MentalIlnessesSet
                                          ] ,
                                          [ rdf:type owl:Restriction ;
                                            owl:onProperty :usedMentalIllnessesSchema ;
                                            owl:qualifiedCardinality "1"^^xsd:nonNegativeInteger ;
                                            owl:onClass :MentalIlnessesSchema
                                          ] ;
                          rdfs:comment "High-level concept used to represent a mental illness detection process regardless of the type (i.e., manual or automatic)." ;
                          rdfs:label "Mental Illnesses Detection"@en ,
                                     "Rilevamento Malattie Mentali"@it .


###  https://w3id.org/miao#MentalIlness
:MentalIlness rdf:type owl:Class ;
              rdfs:subClassOf [ rdf:type owl:Restriction ;
                                owl:onProperty :belongsToMentalIllnessesSet ;
                                owl:qualifiedCardinality "1"^^xsd:nonNegativeInteger ;
                                owl:onClass :MentalIlnessesSet
                              ] ,
                              [ rdf:type owl:Restriction ;
                                owl:onProperty :referredToMentalIllnessCategory ;
                                owl:qualifiedCardinality "1"^^xsd:nonNegativeInteger ;
                                owl:onClass :MentalIlnessCategory
                              ] ;
              rdfs:comment "A MentalIllness represents a detected or predicted mental illness, typically as a result of a human or machine/deep learning analysis." ;
              rdfs:label "Malattia Mentale"@it ,
                         "Mental Illness"@en .


###  https://w3id.org/miao#MentalIlnessCategory
:MentalIlnessCategory rdf:type owl:Class ;
                      rdfs:subClassOf [ rdf:type owl:Restriction ;
                                        owl:onProperty :referredToMentalIllness ;
                                        owl:someValuesFrom :MentalIlness
                                      ] ,
                                      [ rdf:type owl:Restriction ;
                                        owl:onProperty :isMentalIlnessCategoryOf ;
                                        owl:qualifiedCardinality "1"^^xsd:nonNegativeInteger ;
                                        owl:onClass :MentalIlnessesSchema
                                      ] ;
                      rdfs:comment "A concept used to represent a mental illness category that belongs to a specific schema (e.g., ontology) used to represent mental illnesses" ;
                      rdfs:label "Categoria Malattia Mentale"@it ,
                                 "Mental Illness Category"@en .


###  https://w3id.org/miao#MentalIlnessesSchema
:MentalIlnessesSchema rdf:type owl:Class ;
                      rdfs:subClassOf [ rdf:type owl:Restriction ;
                                        owl:onProperty :hasMentalIlnessCategory ;
                                        owl:someValuesFrom :MentalIlnessCategory
                                      ] ,
                                      [ rdf:type owl:Restriction ;
                                        owl:onProperty :usedInMentalIllnessesDetection ;
                                        owl:minQualifiedCardinality "0"^^xsd:nonNegativeInteger ;
                                        owl:onClass :MentalIllnessesDetection
                                      ] ;
                      rdfs:comment "Represents a category of mental illness within a specific schema (e.g., an ontology or classification system)." ;
                      rdfs:label "Mental Illnesses Schema"@en ,
                                 "Schema Malattie Mentali"@it .


###  https://w3id.org/miao#MentalIlnessesSet
:MentalIlnessesSet rdf:type owl:Class ;
                   rdfs:subClassOf <http://www.w3.org/ns/prov#Entity> ,
                                   [ rdf:type owl:Restriction ;
                                     owl:onProperty :hasMentalIllness ;
                                     owl:someValuesFrom :MentalIlness
                                   ] ,
                                   [ rdf:type owl:Restriction ;
                                     owl:onProperty <http://www.w3.org/ns/prov#wasGeneratedBy> ;
                                     owl:qualifiedCardinality "1"^^xsd:nonNegativeInteger ;
                                     owl:onClass :MentalIllnessesDetection
                                   ] ;
                   rdfs:comment "Concept used to represent a set of detected mental illnesses." ;
                   rdfs:label "Insieme Malattie Mentali"@it ,
                              "Mental Illnesses Set"@en .


###  Generated by the OWL API (version 5.1.18) https://github.com/owlcs/owlapi/
