@prefix : <http://www.semanticweb.org/sanar/ontologies/2025/9/MentalIllnessesAnalysisOntology/> .
@prefix owl: <http://www.w3.org/2002/07/owl#> .
@prefix rdf: <http://www.w3.org/1999/02/22-rdf-syntax-ns#> .
@prefix xml: <http://www.w3.org/XML/1998/namespace> .
@prefix xsd: <http://www.w3.org/2001/XMLSchema#> .
@prefix prov: <http://www.w3.org/ns/prov#> .
@prefix rdfs: <http://www.w3.org/2000/01/rdf-schema#> .
@prefix itsrdf: <http://www.w3.org/2005/11/its/rdf#> .
@base <http://www.semanticweb.org/sanar/ontologies/2025/9/MentalIllnessesAnalysisOntology/> .

<http://www.semanticweb.org/sanar/ontologies/2025/9/MentalIllnessesAnalysisOntology> rdf:type owl:Ontology ;
                                                                                      owl:imports <http://www.w3.org/2016/03/mls#> .

#################################################################
#    Object Properties
#################################################################

###  http://www.semanticweb.org/sanar/ontologies/2025/9/MentalIllnessesAnalysisOntology#belongsToMentalIllnessesSet
:belongsToMentalIllnessesSet rdf:type owl:ObjectProperty ;
                             owl:inverseOf :hasMentalIllness ;
                             rdfs:domain :MentalIlness ;
                             rdfs:range :MentalIlnessesSet ;
                             rdfs:comment "Inverse relation of hasMentalIlness. This relation connect a MentalIllness with its corresponding MentalIlnessSet." .


###  http://www.semanticweb.org/sanar/ontologies/2025/9/MentalIllnessesAnalysisOntology#hasMentalIllness
:hasMentalIllness rdf:type owl:ObjectProperty ;
                  rdfs:domain :MentalIlnessesSet ;
                  rdfs:range :MentalIlness ;
                  rdfs:comment "Relation connecting a MentalIllnessSet with its corresponding MentalIlnesses." .


###  http://www.semanticweb.org/sanar/ontologies/2025/9/MentalIllnessesAnalysisOntology#isPredictionOf
:isPredictionOf rdf:type owl:ObjectProperty ;
                owl:inverseOf :hasPrediction ;
                rdfs:domain :Prediction ;
                rdfs:range :PredictionsSet ;
                rdfs:comment "Inverse relation of hasPrediction. This relation connects a Prediction to its correspoding PredictionsSet." .


###  http://www.semanticweb.org/sanar/ontologies/2025/9/MentalIllnessesAnalysisOntology/hasMentalIlness
:hasMentalIlness rdf:type owl:ObjectProperty ;
                 rdfs:subPropertyOf :hasPrediction ;
                 rdfs:domain :MentalIlnessesSet ;
                 rdfs:range :MentalIlness ;
                 rdfs:comment "(Sub)-Relation of hasPrediction object property used to represent the relation between a MentalIllnessesAnalysis and its corresponding MentalIllnesses identified." .


###  http://www.semanticweb.org/sanar/ontologies/2025/9/MentalIllnessesAnalysisOntology/hasMentalIlnessCategory
:hasMentalIlnessCategory rdf:type owl:ObjectProperty ;
                         owl:inverseOf :isMentalIlnessCategoryOf ;
                         rdfs:domain :MentalIlnessesModel ;
                         rdfs:range :MentalIlnessCategory ;
                         rdfs:comment "A relation between a MentalIllnessesModel and its Mental Illnesses categories." .


###  http://www.semanticweb.org/sanar/ontologies/2025/9/MentalIllnessesAnalysisOntology/hasPrediction
:hasPrediction rdf:type owl:ObjectProperty ;
               rdfs:domain :PredictionsSet ;
               rdfs:range :Prediction ;
               rdfs:comment "Relation used to represent the connection between a PredictionsSet and its corresponding Predictions." .


###  http://www.semanticweb.org/sanar/ontologies/2025/9/MentalIllnessesAnalysisOntology/isGeneratedBy
:isGeneratedBy rdf:type owl:ObjectProperty ;
               owl:inverseOf prov:generated ;
               rdf:type owl:InverseFunctionalProperty ;
               rdfs:domain :MentalIlnessesSet ;
               rdfs:range :MentalIlnessesAnalysis ;
               rdfs:comment "Inverse relation of the prov:generated relation. This relation is used to represent the relation between a  MentalIllnessesSet and the MentalIllnessesAnalysis tha generated it." .


###  http://www.semanticweb.org/sanar/ontologies/2025/9/MentalIllnessesAnalysisOntology/isMentalIlnessCategoryOf
:isMentalIlnessCategoryOf rdf:type owl:ObjectProperty ;
                          rdfs:domain :MentalIlnessCategory ;
                          rdfs:range :MentalIlnessesModel ;
                          rdfs:comment "Inverse relation of hasMentalIllnessCategory object propery that represents the relation between a MentalIllnessCategory and its corresponding MentalIllnessesModel." .


###  http://www.semanticweb.org/sanar/ontologies/2025/9/MentalIllnessesAnalysisOntology/referredToMentalIllness
:referredToMentalIllness rdf:type owl:ObjectProperty ;
                         owl:inverseOf :referredToMentalIllnessCategory ;
                         rdf:type owl:InverseFunctionalProperty ;
                         rdfs:domain :MentalIlnessCategory ;
                         rdfs:range :MentalIlness ;
                         rdfs:comment "Inverse relation of referredToMentalIllnessCategory used to represent to which MentalIlness (predicted) a MentalIlnessCategoy (from the literature) corresponds to." .


###  http://www.semanticweb.org/sanar/ontologies/2025/9/MentalIllnessesAnalysisOntology/referredToMentalIllnessCategory
:referredToMentalIllnessCategory rdf:type owl:ObjectProperty ,
                                          owl:FunctionalProperty ;
                                 rdfs:domain :MentalIlness ;
                                 rdfs:range :MentalIlnessCategory ;
                                 rdfs:comment "Relation used to represent to which MentalIlnessCategoy (from the literature) a MentalIlness (predicted) corresponds to." .


###  http://www.semanticweb.org/sanar/ontologies/2025/9/MentalIllnessesAnalysisOntology/usedInMentalIlnessesAnalysis
:usedInMentalIlnessesAnalysis rdf:type owl:ObjectProperty ;
                              rdfs:domain :MentalIlnessesModel ;
                              rdfs:range :MentalIlnessesAnalysis ;
                              rdfs:comment "Inverse relation of usedMentalIlnessesAnalysis used to indicate which MetalIllnessAnalysis adopted a specific MentalIllnessesModel (from the literature)." .


###  http://www.semanticweb.org/sanar/ontologies/2025/9/MentalIllnessesAnalysisOntology/usedMentalIlnessesModel
:usedMentalIlnessesModel rdf:type owl:ObjectProperty ,
                                  owl:FunctionalProperty ;
                         rdfs:domain :MentalIlnessesAnalysis ;
                         rdfs:range :MentalIlnessesModel ;
                         rdfs:comment "Relations used to indicate to which MentalIllnessesModel (from the literature) a MentalIllnessesAnalysis is based on." .


###  http://www.w3.org/ns/prov#generated
prov:generated rdf:type owl:ObjectProperty ,
                        owl:FunctionalProperty ;
               rdfs:domain :MentalIlnessesAnalysis ;
               rdfs:range :MentalIlnessesSet ;
               rdfs:comment "Relation taken from the Prov ontology that is used to represent the relation between a MentalIlness Analysis and the generated set of MentalIllnessesSet." .


#################################################################
#    Data properties
#################################################################

###  http://www.semanticweb.org/sanar/ontologies/2025/9/MentalIllnessesAnalysisOntology/MLConfidence
:MLConfidence rdf:type owl:DatatypeProperty ;
              rdfs:domain :Prediction ;
              rdfs:range xsd:decimal ;
              rdfs:comment "Data Property used to represent the confidence of a machine/deep learning model." .


###  http://www.semanticweb.org/sanar/ontologies/2025/9/MentalIllnessesAnalysisOntology/hasMentalIllnessLevel
:hasMentalIllnessLevel rdf:type owl:DatatypeProperty ;
                       rdfs:domain :MentalIlness ;
                       rdfs:range xsd:string ;
                       rdfs:comment "Represents the intensity of the mental illness as a categorical value, e.g., Low, Medium, or High." .


###  http://www.semanticweb.org/sanar/ontologies/2025/9/MentalIllnessesAnalysisOntology/hasMentalIllnessScore
:hasMentalIllnessScore rdf:type owl:DatatypeProperty ;
                       rdfs:domain :MentalIlness ;
                       rdfs:range xsd:decimal ;
                       rdfs:comment "Represents the intensity of the mental illness as a numeric score between 0 and 1." .


#################################################################
#    Classes
#################################################################

###  http://www.semanticweb.org/sanar/ontologies/2025/9/MentalIllnessesAnalysisOntology/DisorderType
:DisorderType rdf:type owl:Class ;
              rdfs:subClassOf :MentalIlness ;
              rdfs:comment "This concept defines the types of disorder(s) related to a MentalIllness." ;
              rdfs:label "Disorder type"@en ,
                         "Tipo disordine"@it .


###  http://www.semanticweb.org/sanar/ontologies/2025/9/MentalIllnessesAnalysisOntology/MentalIlness
:MentalIlness rdf:type owl:Class ;
              rdfs:subClassOf :Prediction ,
                              [ rdf:type owl:Restriction ;
                                owl:onProperty :belongsToMentalIllnessesSet ;
                                owl:someValuesFrom :MentalIlnessesSet
                              ] ,
                              [ rdf:type owl:Restriction ;
                                owl:onProperty :referredToMentalIllnessCategory ;
                                owl:qualifiedCardinality "1"^^xsd:nonNegativeInteger ;
                                owl:onClass :MentalIlnessCategory
                              ] ;
              rdfs:comment "A concept used to represent the result (i.e., a prediction) from a machine/deep learning model." ;
              rdfs:label "Malattia Mentale"@it ,
                         "Mental Illness"@en .


###  http://www.semanticweb.org/sanar/ontologies/2025/9/MentalIllnessesAnalysisOntology/MentalIlnessCategory
:MentalIlnessCategory rdf:type owl:Class ;
                      rdfs:subClassOf [ rdf:type owl:Restriction ;
                                        owl:onProperty :isMentalIlnessCategoryOf ;
                                        owl:qualifiedCardinality "1"^^xsd:nonNegativeInteger ;
                                        owl:onClass :MentalIlnessesModel
                                      ] ,
                                      [ rdf:type owl:Restriction ;
                                        owl:onProperty :referredToMentalIllness ;
                                        owl:qualifiedCardinality "1"^^xsd:nonNegativeInteger ;
                                        owl:onClass :MentalIlness
                                      ] ;
                      rdfs:comment "A concept used to represent a mental illness category that belongs to a specific model (e.g., ontology) used to represent mental illnesses" ;
                      rdfs:label "Categoria Malattia Mentale"@it ,
                                 "Mental Illness Category"@en .


###  http://www.semanticweb.org/sanar/ontologies/2025/9/MentalIllnessesAnalysisOntology/MentalIlnessesAnalysis
:MentalIlnessesAnalysis rdf:type owl:Class ;
                        rdfs:subClassOf <http://www.w3.org/ns/mls#Run> ,
                                        prov:Activity ,
                                        [ rdf:type owl:Restriction ;
                                          owl:onProperty :usedMentalIlnessesModel ;
                                          owl:qualifiedCardinality "1"^^xsd:nonNegativeInteger ;
                                          owl:onClass :MentalIlnessesModel
                                        ] ,
                                        [ rdf:type owl:Restriction ;
                                          owl:onProperty prov:generated ;
                                          owl:qualifiedCardinality "1"^^xsd:nonNegativeInteger ;
                                          owl:onClass :MentalIlnessesSet
                                        ] ;
                        rdfs:comment "A Mental Illness Analysis represent an analysis (i.e., a run) of a machine/deep learning model to discover the presence of mental ilnesses from a given source." ;
                        rdfs:label "Analisi Malattie Mentali"@it ,
                                   "Mental Illnesses Analysis"@en .


###  http://www.semanticweb.org/sanar/ontologies/2025/9/MentalIllnessesAnalysisOntology/MentalIlnessesModel
:MentalIlnessesModel rdf:type owl:Class ;
                     rdfs:subClassOf [ rdf:type owl:Restriction ;
                                       owl:onProperty :hasMentalIlnessCategory ;
                                       owl:someValuesFrom :MentalIlnessCategory
                                     ] ,
                                     [ rdf:type owl:Restriction ;
                                       owl:onProperty :usedInMentalIlnessesAnalysis ;
                                       owl:someValuesFrom :MentalIlnessesAnalysis
                                     ] ;
                     rdfs:comment "A Mental Ilnesses Model represents a model (from literature) used to represent mental illnesses (e.g., an ontology)." ;
                     rdfs:label "Mental Illnesses Model"@en .


###  http://www.semanticweb.org/sanar/ontologies/2025/9/MentalIllnessesAnalysisOntology/MentalIlnessesSet
:MentalIlnessesSet rdf:type owl:Class ;
                   rdfs:subClassOf :PredictionsSet ,
                                   [ rdf:type owl:Restriction ;
                                     owl:onProperty :hasMentalIllness ;
                                     owl:someValuesFrom :MentalIlness
                                   ] ,
                                   [ rdf:type owl:Restriction ;
                                     owl:onProperty :isGeneratedBy ;
                                     owl:qualifiedCardinality "1"^^xsd:nonNegativeInteger ;
                                     owl:onClass :MentalIlnessesAnalysis
                                   ] ;
                   rdfs:label "Insieme Malattie Mentali"@it ,
                              "Mental Illnesses Set"@en .


###  http://www.semanticweb.org/sanar/ontologies/2025/9/MentalIllnessesAnalysisOntology/Prediction
:Prediction rdf:type owl:Class ;
            rdfs:subClassOf [ rdf:type owl:Restriction ;
                              owl:onProperty :isPredictionOf ;
                              owl:someValuesFrom :PredictionsSet
                            ] ;
            rdfs:comment "Prediction represents a prediction from a machine/deep learning model." ;
            rdfs:label "Prediction"@en ,
                       "Predizione"@it .


###  http://www.semanticweb.org/sanar/ontologies/2025/9/MentalIllnessesAnalysisOntology/PredictionsSet
:PredictionsSet rdf:type owl:Class ;
                rdfs:subClassOf [ rdf:type owl:Restriction ;
                                  owl:onProperty :hasPrediction ;
                                  owl:someValuesFrom :Prediction
                                ] ;
                rdfs:comment "Predictions Set is a concept used to collect (multiple) Predictions from a machine/deep learning model." ;
                rdfs:label "Insieme Predizioni"@it ,
                           "Predictions Set"@en .


###  http://www.w3.org/ns/prov#Activity
prov:Activity rdf:type owl:Class ;
              rdfs:comment "Ref: https://www.w3.org/TR/prov-o/#Activity" .


###  Generated by the OWL API (version 4.5.25.2023-02-15T19:15:49Z) https://github.com/owlcs/owlapi
